

Sample

November 22, 2025

1 Preamble / Introduction

The point $(1, -2)$ is on the graph of f . Describe the following transformations on f , and determine the resulting point. We use $g(x) = a f k(x - d) + c$, $x' = x k + d$, $y' = a y + c$. a) $g(x) = 2f(x) + 3$ The $a = 2$ indicates a vertical stretch by a factor of 2 and the $c = 3$ indicates a vertical translation of 3 units up. $x' = x k + d = 1 \cdot 1 + 0 = 1$ $y' = a y + c = 2(-2) + 3 = -1$ Therefore, the resulting point is $(1, -1)$. 6 b) $g(x) = f(x + 1) - 3$ The $d = -1$ (since $x - d = x - (-1) = x + 1$) indicates a horizontal translation of 1 unit to the left and the $c = -3$ indicates a vertical translation of 3 units down. $x' = x k + d = 1 \cdot 1 + (-1) = 0$ $y' = a y + c = 1(-2) + (-3) = -5$ Therefore, the resulting point is $(0, -5)$. c) $g(x) = -f(2x)$ The $a = -1$ indicates a reflection in the x -axis and the $k = 2$ indicates a horizontal compression by a factor of $1/2$. $x' = x k + d = 1 \cdot 2 + 0 = 2$ $y' = a y + c = (-1)(-2) + 0 = 2$ Therefore, the resulting point is $(2, 2)$. 7 d) $g(x) = -f(-x - 1) + 3$ The $a = -1$ indicates a reflection in the x -axis, the $k = -1$ indicates a reflection in the y -axis, the $d = -1$ (from $x - d = x - (-1) = x + 1$) indicates a horizontal translation of 1 unit to the left, and the $c = 3$ indicates a vertical translation of 3 units up. $x' = x k + d = 1 \cdot (-1) + (-1) = -2$ $y' = a y + c = (-1)(-2) + 3 = 5$ Therefore, the resulting point is $(-2, 5)$. 8 The point $(1, -2)$ is on the graph of f . Describe the following transformations on f , and determine the resulting point. We use $g(x) = a f k(x - d) + c$, $x' = x k + d$, $y' = a y + c$. a) $g(x) = 2f(x) + 3$ The $a = 2$ indicates a vertical stretch by a factor of 2 and the $c = 3$ indicates a vertical translation of 3 units up. $x' = x k + d = 1 \cdot 1 + 0 = 1$ $y' = a y + c = 2(-2) + 3 = -1$ Therefore, the resulting point is $(1, -1)$. 6 b) $g(x) = f(x + 1) - 3$ The $d = -1$ (since $x - d = x - (-1) = x + 1$) indicates a horizontal translation of 1 unit to the left and the $c = -3$ indicates a vertical translation of 3 units down. $x' = x k + d = 1 \cdot 1 + (-1) = 0$ $y' = a y + c = 1(-2) + (-3) = -5$ Therefore, the resulting point is $(0, -5)$. c) $g(x) = -f(2x)$ The $a = -1$ indicates a reflection in the x -axis and the $k = 2$ indicates a horizontal compression by a factor of $1/2$. $x' = x k + d = 1 \cdot 2 + 0 = 2$ $y' = a y + c = (-1)(-2) + 0 = 2$ Therefore, the resulting point is $(2, 2)$. 7 d) $g(x) = -f(-x - 1) + 3$ The $a = -1$ indicates a reflection in the x -axis, the $k = -1$ indicates a reflection in the y -axis, the $d = -1$ (from $x - d = x - (-1) = x + 1$) indicates a horizontal translation of 1 unit to the left, and the $c = 3$ indicates a vertical translation of 3 units up. $x' = x k + d = 1 \cdot (-1) + (-1) = -2$ $y' = a y + c = (-1)(-2) + 3 = 5$ Therefore, the resulting point is $(-2, 5)$. 8 The point $(1, -2)$ is on the graph of f . Describe the following transformations on f , and determine the resulting point. We use $g(x) = a f k(x - d) + c$, $x' = x k + d$, $y' = a y + c$. a) $g(x) = 2f(x) + 3$ The $a = 2$ indicates a vertical stretch by a factor of 2 and the $c = 3$ indicates a vertical translation of 3 units up. $x' = x k + d = 1 \cdot 1 + 0 = 1$ $y' = a y + c = 2(-2) + 3 = -1$ Therefore, the resulting point is $(1, -1)$. 6 b) $g(x) = f(x + 1) - 3$ The $d = -1$ (since $x - d = x - (-1) = x + 1$) indicates a horizontal

2

reflection in the y-axis, the $d = -1$ (from $x - d = x - (-1) = x + 1$) indicates a horizontal translation of 1 unit to the left, and the $c = 3$ indicates a vertical translation of 3 units up. $x' = x k + d = 1 \cdot (-1) + (-1) = -2$ $y' = a y + c = (-1)(-2) + 3 = 5$ Therefore, the resulting point is $(-2, 5)$. 8 The point $(1, -2)$ is on the graph of f . Describe the following transformations on f , and determine the resulting point. We use $g(x) = a f k(x - d) + c$, $x' = x k + d$, $y' = a y + c$. a) $g(x) = 2f(x) + 3$ The $a = 2$ indicates a vertical stretch by a factor of 2 and the $c = 3$ indicates a vertical translation of 3 units up. $x' = x k + d = 1 \cdot 1 + 0 = 1$ $y' = a y + c = 2(-2) + 3 = -1$ Therefore, the resulting point is $(1, -1)$. 6 b) $g(x) = f(x + 1) - 3$ The $d = -1$ (since $x - d = x - (-1) = x + 1$) indicates a horizontal translation of 1 unit to the left and the $c = -3$ indicates a vertical translation of 3 units down. $x' = x k + d = 1 \cdot 1 + (-1) = 0$ $y' = a y + c = 1(-2) + (-3) = -5$ Therefore, the resulting point is $(0, -5)$. c) $g(x) = -f(2x)$ The $a = -1$ indicates a reflection in the x-axis and the $k = 2$ indicates a horizontal compression by a factor of $1/2$. $x' = x k + d = 1 \cdot 2 + 0 = 2$ $y' = a y + c = (-1)(-2) + 0 = 2$ Therefore, the resulting point is $(2, 2)$. d) $g(x) = -f(-x - 1) + 3$ The $a = -1$ indicates a reflection in the x-axis, the $k = -1$ indicates a reflection in the y-axis, the $d = -1$ (from $x - d = x - (-1) = x + 1$) indicates a horizontal translation of 1 unit to the left, and the $c = 3$ indicates a vertical translation of 3 units up. $x' = x k + d = 1 \cdot (-1) + (-1) = -2$ $y' = a y + c = (-1)(-2) + 3 = 5$ Therefore, the resulting point is $(-2, 5)$. 8 The point $(1, -2)$ is on the graph of f . Describe the following transformations on f , and determine the resulting point. We use $g(x) = a f k(x - d) + c$, $x' = x k + d$, $y' = a y + c$. a) $g(x) = 2f(x) + 3$ The $a = 2$ indicates a vertical stretch by a factor of 2 and the $c = 3$ indicates a vertical translation of 3 units up. $x' = x k + d = 1 \cdot 1 + 0 = 1$ $y' = a y + c = 2(-2) + 3 = -1$ Therefore, the resulting point is $(1, -1)$. 6 b) $g(x) = f(x + 1) - 3$ The $d = -1$ (since $x - d = x - (-1) = x + 1$) indicates a horizontal translation of 1 unit to the left and the $c = -3$ indicates a vertical translation of 3 units down. $x' = x k + d = 1 \cdot 1 + (-1) = 0$ $y' = a y + c = 1(-2) + (-3) = -5$ Therefore, the resulting point is $(0, -5)$. c) $g(x) = -f(2x)$ The $a = -1$ indicates a reflection in the x-axis and the $k = 2$ indicates a horizontal compression by a factor of $1/2$. $x' = x k + d = 1 \cdot 2 + 0 = 2$ $y' = a y + c = (-1)(-2) + 0 = 2$ Therefore, the resulting point is $(2, 2)$. d) $g(x) = -f(-x - 1) + 3$ The $a = -1$ indicates a reflection in the x-axis, the $k = -1$ indicates a reflection in the y-axis, the $d = -1$ (from $x - d = x - (-1) = x + 1$) indicates a horizontal translation of 1 unit to the left, and the $c = 3$ indicates a vertical translation of 3 units up. $x' = x k + d = 1 \cdot (-1) + (-1) = -2$ $y' = a y + c = (-1)(-2) + 3 = 5$ Therefore, the resulting point is $(-2, 5)$. 8 The point $(1, -2)$ is on the graph of f . Describe the following transformations on f , and determine the resulting point. We use $g(x) = a f k(x - d) + c$, $x' = x k + d$, $y' = a y + c$. a) $g(x) = 2f(x) + 3$ The $a = 2$ indicates a vertical stretch by a factor

of 2 and the $c = 3$ indicates a vertical translation of 3 units up. $x' = x k + d = 1 \cdot 1 + 0 = 1$ $y' = a y + c = 2(-2) + 3 = -1$ Therefore, the resulting point is $(1, -1)$. 6 b) $g(x) = f(x + 1) - 3$ The $d = -1$ (since $x - d = x - (-1) = x + 1$) indicates a horizontal translation of 1 unit to the left and the $c = -3$ indicates a vertical translation of 3 units down. $x' = x k + d = 1 \cdot 1 + (-1) = 0$ $y' = a y + c = 1(-2) + (-3) = -5$ Therefore, the resulting point is $(0, -5)$. c) $g(x) = -f(2x)$ The $a = -1$ indicates a reflection in the x-axis and the $k = 2$ indicates a horizontal compression by a factor of $1/2$. $x' = x k + d = 1 \cdot 2 + 0 = 2$ $y' = a y + c = (-1)(-2) + 0 = 2$ Therefore, the resulting point is $(2, 2)$. 7 d) $g(x) = -f(-x - 1) + 3$ The $a = -1$ indicates a reflection in the x-axis, the $k = -1$ indicates a reflection in the y-axis, the $d = -1$ (from $x - d = x - (-1) = x + 1$) indicates a horizontal translation of 1 unit to the left, and the $c = 3$ indicates a vertical translation of 3 units up. $x' = x k + d = 1 \cdot (-1) + (-1) = -2$ $y' = a y + c = (-1)(-2) + 3 = 5$ Therefore, the resulting point is $(-2, 5)$. 8 The point $(1, -2)$ is on the graph of f . Describe the following transformations on f , and determine the resulting point. We use $g(x) = a f(k(x - d)) + c$, $x' = x k + d$, $y' = a y + c$. a) $g(x) = 2f(x) + 3$ The $a = 2$ indicates a vertical stretch by a factor of 2 and the $c = 3$ indicates a vertical translation of 3 units up. $x' = x k + d = 1 \cdot 1 + 0 = 1$ $y' = a y + c = 2(-2) + 3 = -1$ Therefore, the resulting point is $(1, -1)$. 6 b) $g(x) = f(x + 1) - 3$ The $d = -1$ (since $x - d = x - (-1) = x + 1$) indicates a horizontal translation of 1 unit to the left and the $c = -3$ indicates a vertical translation of 3 units down. $x' = x k + d = 1 \cdot 1 + (-1) = 0$ $y' = a y + c = 1(-2) + (-3) = -5$ Therefore, the resulting point is $(0, -5)$. c) $g(x) = -f(2x)$ The $a = -1$ indicates a reflection in the x-axis and the $k = 2$ indicates a horizontal compression by a factor of $1/2$. $x' = x k + d = 1 \cdot 2 + 0 = 2$ $y' = a y + c = (-1)(-2) + 0 = 2$ Therefore, the resulting point is $(2, 2)$. 7 d) $g(x) = -f(-x - 1) + 3$ The $a = -1$ indicates a reflection in the x-axis, the $k = -1$ indicates a reflection in the y-axis, the $d = -1$ (from $x - d = x - (-1) = x + 1$) indicates a horizontal translation of 1 unit to the left, and the $c = 3$ indicates a vertical translation of 3 units up. $x' = x k + d = 1 \cdot (-1) + (-1) = -2$ $y' = a y + c = (-1)(-2) + 3 = 5$ Therefore, the resulting point is $(-2, 5)$. 8